benchmarks/sorting/eval_benchmark.sh
@@ -1,9 +1,12 @@
 #!/bin/bash
 
-rm ~/tmp/data*.tex
+# LOG="log/all-2020-10-09.log"
+LOG="log/test.log"
+
+rm -rf ~/tmp/data*.tex
 
 # cat log/sortbench-2020-01-all.log | ./__eval_benchmark.awk > /tmp/data.tex
-cat log/all-2020-10-09.log | ./__eval_benchmark.awk > ~/tmp/data.tex
+cat $LOG | ./__eval_benchmark.awk > ~/tmp/data.tex
 
 gawk '$1=="@" { echo=($2=="introsort"); next }  echo {print} ' ~/tmp/data.tex  > ~/tmp/data_introsort.tex
 # gawk '$1=="@" { echo=($2=="pdqsort"); next }  echo {print} ' ~/tmp/data.tex > ~/tmp/data_pdqsort.tex
